\chapter{Feb.~26 --- Dispersive Decay with Potential, Part 3}

\section{Low Energy Estimates, Continued}
\begin{proof}[Proof of Lemma \ref{lem:low-energy}, continued]
  Our goal is to understand $f_\pm$. Define
  $m_+(\lambda, x) = e^{i\lambda x} f_+(\lambda)$,
  so that
  \[
    m_+(\lambda, x) \to 1 \quad \text{as $x \to \infty$}
  \]
  ``Volterra iteration'' gives more precise
  estimates, but we will go with a rougher approach:
  $m_+$ satisfies
  \[
    \partial_x^2 m_+(\lambda, x) + 2i \lambda \partial_x m_+(\lambda, x) + V(x) m_+(\lambda, x) = 0.
  \]
  Then we have the \emph{Volterra equation}
  \[
    m_+(\lambda, x) = 1 + \int_x^\infty D_\lambda(x - y) V(y) m_+(\lambda, y)\, dy, \quad
    D_\lambda = \int_0^x e^{2i\lambda z}\, dz = \frac{e^{2i\lambda x} - 1}{2 i \lambda}.
  \]
  Denote $\dot{m}_+(\lambda, x) = \partial_\lambda m_+(\lambda, x)$
  and $\ddot{m}_+(\lambda, x) = \partial_\lambda^2 m_+(\lambda, x)$,
  which satisfy
  \[
    \dot{m}_+(\lambda, x) = \int_x^\infty D_\lambda(x - y) V(y) \dot{m}_+(\lambda, y)\, dy
    + \int_x^\infty \dot{D}_\lambda(x - y) V(y) m_+(\lambda, y)\, dy
  \]
  and a similar integral equation for $\ddot{m}_+$. We
  want to
  show the existence of $m_+$, and we are interested
  in the behavior of $m_+$ as $x \to \infty$.
  We will solve the equation on $[x_0, \infty)$ for
  $x_0$ large enough. Set
  \[
    z_+(\lambda, x)
    = \langle \lambda \rangle \frac{m_+(k, x) - 1}{W_+'(x)}, \quad
    W_+'(x) = \int_x^\infty \langle y \rangle |V(y)|\, dy.
  \]
  where $\langle \lambda \rangle = \sqrt{1 + \lambda^2}$
  is the \emph{Japanese bracket}.
  Note that $W_+'(x) \to 0$ with the same rate, and if
  \[
    \int \langle y \rangle^n |V(y)|\, dy < \infty,
  \]
  then $|W_+'(x)| \le \langle x \rangle^{1 - n}$.
  From the equation of $m_+$, we can see that
  \[
    (I - L) z_+(k, x) = z_+(k, x) - L z_+
    = \frac{\langle \lambda \rangle}{W_+'(x)} \int_x^\infty D_\lambda(y - x) V(y)\, dy, \quad
  \]
  where $Lz_+$ is given by
  \[
    L z_+ = \frac{1}{W_+'(x)} \int_x^\infty D_\lambda(y - x) V(y) W_+'(y) z_+(y) \, dy.
  \]
  Our goal is to show that $(I - L)$ is invertible
  on $L^\infty([x_0, \infty))$.
  Note that we have
  $|D_\lambda(z)| \lesssim |z| / |\lambda|$
  since $|e^{ix} - 1| \le |x|$, and also
  $|D_\lambda(z)| \le |z|$. Then we can estimate
  \[
    \left\|\langle \lambda \rangle W_+' \int_x^\infty D_\lambda(y - x) V(y)\, dy \right\|_{L^\infty([x_0, \infty))}
    \lesssim
    \left\|\langle \lambda \rangle W_+' \int_x^\infty \frac{|y - x|}{|\lambda|} V(y)\, dy \right\|_{L^\infty([x_0, \infty))}
    < \infty
  \]
  So if $(I - L) z_+ = G$, then from the
  above computation $\|G\|_{L^\infty([x_0, \infty))} < \infty$.
  We also have
  \begin{align*}
    \|Lz_+\|_{L^\infty([x_0, \infty))}
    &\lesssim \left\|\frac{1}{W_+'(x)} \int_x^\infty |y - x| V(y) W_+'(y) \|z_+\|_{L^\infty}\, dy \right\|_{L^\infty([x_0, \infty))} \\
    &\lesssim W_+'(x_0) \|z_+\|_{L^\infty([x_0, \infty))}\left\|\frac{1}{W_+'(x)} \int_x^\infty |y - x| |V(y)|\, dy \right\|_{L^\infty([x_0, \infty))} \\
    &\lesssim W_+'(x_0) \|z_+\|_{L^\infty([x_0, \infty))}.
  \end{align*}
  As $|x_0| \to \infty$, we have
  $\|Lz_+\|_{L^\infty([x_0, \infty))} \ll \|z_+\|_{L^\infty([x_0, \infty))}$,
  so $(I - L)$ is invertible on
  $L^\infty([x_0, \infty))$. Thus $z_+$ exists
  in $L^\infty([x_0, \infty))$, hence
  $m_+$ also exists in $L^\infty([x_0, \infty))$.

  We still need to work on $(-\infty, x_0)$.
  For $-1 \le x \le x_0$, we have
  \[
    |z_+(\lambda, x)|
    \lesssim 1 + \int_x^{x_0} \langle y \rangle |V(y)| |z_+(\lambda, y)|\, dy,
  \]
  so by Gronwall's inequality,
  $|z_+(\lambda, x)| \lesssim 1$. For $x \le 0$,
  we can notice that
  \[
    \frac{|z_+(\lambda, x)|}{\langle x \rangle}
    \lesssim 1 + \frac{1}{\langle x \rangle} \int_x^0 \langle x - y\rangle |V(y)| \frac{|z_+(\lambda, y)|}{\langle y \rangle}\, dy
    \lesssim 1 + \int_x^0 \langle y\rangle |V(y)| \frac{|z_+(\lambda, y)|}{\langle y \rangle}\, dy
  \]
  Applying Gronwall's inequality again, we obtain
  $|z_+(\lambda, x) / \langle x \rangle| \lesssim 1$.\footnote{Note that one can also apply Gronwall's inequality for $x > 0$, but the resulting estimate $|z_+(\lambda, x)| \lesssim \langle x \rangle$ does not give precise asymptotic information for $z_+$ as $x \to \infty$.}
  So we know the existence of $f_+$ and $m_+$, and
  a similar argument shows the existence of
  $f_-$ and $m_-$. We can also obtain estimates for
  $\dot{m}_\pm$ and $\ddot{m}_\pm$ in a similar fashion.
  We continue the proof from here next time.
\end{proof}

\begin{remark}
  Inserting the formula for $m_+$ again in the
  Volterra equation yields
  \begin{align*}
    m_+(\lambda, x)
    &= 1 + \int_x^\infty D_\lambda(x - y) V(y) m_+(\lambda, y)\, dy \\
    &= 1 + \int_x^\infty D_\lambda(x - y) V(y) \, dy
    + \int_x^\infty D_\lambda(x - y) V(y) \int_y^\infty D_\lambda(y - z) V(z) m_+(\lambda, z)\, dz\, dy \\
    &= \dots.
  \end{align*}
  Iterating this process (Volterra iteration) and
  bounding each term not
  involving $m_+$ gives more precise estimates (argue
  that one ends up with a summable series and get
  estimates from there).
\end{remark}

\begin{lemma}
  Suppose $W(0) \ne 0$. Then we have
  \[
    \sup_{x < y} \left|\int_{-\infty}^\infty e^{it\lambda^2} \frac{\lambda \chi(x^2)}{W(\lambda)} f_+(\lambda)\ f_-(\lambda, x), d\lambda\right|
    \le |t|^{-1 / 2}.
  \]
\end{lemma}
